fstar/MLS.TreeSync.Invariants.AuthService.Proofs.fst
@@ -13,14 +13,14 @@ open MLS.TreeSync.Invariants.AuthService
 
 #set-options "--fuel 1 --ifuel 1"
 
-val intro_all_credentials_ok: #bytes:Type0 -> {|bytes_like bytes|} -> #tkt:treekem_types bytes -> #asp:as_parameters bytes -> #l:nat -> #i:tree_index l -> ts:treesync bytes tkt l i -> ast:as_tokens bytes asp l i -> (li:leaf_index l i -> squash (one_credential_ok ts ast li)) -> squash (all_credentials_ok ts ast)
+val intro_all_credentials_ok: #bytes:Type0 -> {|bytes_like bytes|} -> #tkt:treekem_types bytes -> #asp:as_parameters bytes -> #l:nat -> #i:tree_index l -> ts:treesync bytes tkt l i -> ast:as_tokens bytes asp.token_t l i -> (li:leaf_index l i -> squash (one_credential_ok ts ast li)) -> squash (all_credentials_ok ts ast)
 let intro_all_credentials_ok #bytes #bl #tkt #asp #l #i ts ast one_proof =
   introduce forall li. one_credential_ok ts ast li
   with one_proof li
 
 (*** Invariant theorems ***)
 
-val all_credentials_ok_tree_add: #bytes:Type0 -> {|bytes_like bytes|} -> #tkt:treekem_types bytes -> #asp:as_parameters bytes -> #l:nat -> #i:tree_index l -> ts:treesync bytes tkt l i -> ast:as_tokens bytes asp l i -> li:leaf_index l i -> ln:leaf_node_nt bytes tkt -> token:asp.token_t -> Lemma
+val all_credentials_ok_tree_add: #bytes:Type0 -> {|bytes_like bytes|} -> #tkt:treekem_types bytes -> #asp:as_parameters bytes -> #l:nat -> #i:tree_index l -> ts:treesync bytes tkt l i -> ast:as_tokens bytes asp.token_t l i -> li:leaf_index l i -> ln:leaf_node_nt bytes tkt -> token:asp.token_t -> Lemma
   (requires
     asp.credential_ok (ln.data.signature_key, ln.data.credential) token /\
     all_credentials_ok ts ast /\
@@ -33,7 +33,7 @@ let all_credentials_ok_tree_add #bytes #bl #tkt #asp #l #i ts ast li ln token =
     leaf_at_tree_change_path ast li (Some token) () li'
   )
 
-val all_credentials_ok_tree_update: #bytes:Type0 -> {|bytes_like bytes|} -> #tkt:treekem_types bytes -> #asp:as_parameters bytes -> #l:nat -> #i:tree_index l -> ts:treesync bytes tkt l i -> ast:as_tokens bytes asp l i -> li:leaf_index l i -> ln:leaf_node_nt bytes tkt -> token:asp.token_t -> Lemma
+val all_credentials_ok_tree_update: #bytes:Type0 -> {|bytes_like bytes|} -> #tkt:treekem_types bytes -> #asp:as_parameters bytes -> #l:nat -> #i:tree_index l -> ts:treesync bytes tkt l i -> ast:as_tokens bytes asp.token_t l i -> li:leaf_index l i -> ln:leaf_node_nt bytes tkt -> token:asp.token_t -> Lemma
   (requires
     asp.credential_ok (ln.data.signature_key, ln.data.credential) token /\
     all_credentials_ok ts ast
@@ -45,7 +45,7 @@ let all_credentials_ok_tree_update #bytes #bl #tkt #asp #l #i ts ast li ln token
     leaf_at_tree_change_path ast li (Some token) () li'
   )
 
-val all_credentials_ok_tree_remove: #bytes:Type0 -> {|bytes_like bytes|} -> #tkt:treekem_types bytes -> #asp:as_parameters bytes -> #l:nat -> #i:tree_index l -> ts:treesync bytes tkt l i -> ast:as_tokens bytes asp l i -> li:leaf_index l i -> Lemma
+val all_credentials_ok_tree_remove: #bytes:Type0 -> {|bytes_like bytes|} -> #tkt:treekem_types bytes -> #asp:as_parameters bytes -> #l:nat -> #i:tree_index l -> ts:treesync bytes tkt l i -> ast:as_tokens bytes asp.token_t l i -> li:leaf_index l i -> Lemma
   (requires all_credentials_ok ts ast)
   (ensures all_credentials_ok (tree_remove ts li) (as_remove ast li))
 let all_credentials_ok_tree_remove #bytes #bl #tkt #asp #l #i ts ast li =
@@ -54,7 +54,7 @@ let all_credentials_ok_tree_remove #bytes #bl #tkt #asp #l #i ts ast li =
     leaf_at_tree_change_path ast li None () li'
   )
 
-val all_credentials_ok_apply_path: #bytes:Type0 -> {|crypto_bytes bytes|} -> #tkt:treekem_types bytes -> #asp:as_parameters bytes -> #l:nat -> #li:leaf_index l 0 -> ts:treesync bytes tkt l 0 -> ast:as_tokens bytes asp l 0 -> p:pathsync bytes tkt l 0 li -> token:asp.token_t -> Lemma
+val all_credentials_ok_apply_path: #bytes:Type0 -> {|crypto_bytes bytes|} -> #tkt:treekem_types bytes -> #asp:as_parameters bytes -> #l:nat -> #li:leaf_index l 0 -> ts:treesync bytes tkt l 0 -> ast:as_tokens bytes asp.token_t l 0 -> p:pathsync bytes tkt l 0 li -> token:asp.token_t -> Lemma
   (requires
     asp.credential_ok ((get_path_leaf p).data.signature_key, (get_path_leaf p).data.credential) token /\
     all_credentials_ok ts ast /\
@@ -67,7 +67,7 @@ let all_credentials_ok_apply_path #bytes #cb #tkt #asp #l #li ts ast p token =
     leaf_at_tree_change_path ast li (Some token) () li'
   )
 
-val all_credentials_ok_left_right: #bytes:Type0 -> {|bytes_like bytes|} -> #tkt:treekem_types bytes -> #asp:as_parameters bytes -> #l:pos -> #i:tree_index l -> ts:treesync bytes tkt l i -> ast:as_tokens bytes asp l i -> Lemma
+val all_credentials_ok_left_right: #bytes:Type0 -> {|bytes_like bytes|} -> #tkt:treekem_types bytes -> #asp:as_parameters bytes -> #l:pos -> #i:tree_index l -> ts:treesync bytes tkt l i -> ast:as_tokens bytes asp.token_t l i -> Lemma
   (requires all_credentials_ok ts ast)
   (ensures (
     let TNode _ ts_left ts_right, TNode _ ast_left ast_right = ts, ast in
@@ -86,13 +86,13 @@ let all_credentials_ok_left_right #bytes #bl #tkt #asp #l #i ts ast =
     assert(leaf_at ast_right li == leaf_at ast li)
   )
 
-val all_credentials_ok_tree_truncate: #bytes:Type0 -> {|bytes_like bytes|} -> #tkt:treekem_types bytes -> #asp:as_parameters bytes -> #l:pos -> ts:treesync bytes tkt l 0 -> ast:as_tokens bytes asp l 0 -> Lemma
+val all_credentials_ok_tree_truncate: #bytes:Type0 -> {|bytes_like bytes|} -> #tkt:treekem_types bytes -> #asp:as_parameters bytes -> #l:pos -> ts:treesync bytes tkt l 0 -> ast:as_tokens bytes asp.token_t l 0 -> Lemma
   (requires all_credentials_ok ts ast /\ is_tree_empty (TNode?.right ts))
   (ensures all_credentials_ok (tree_truncate ts) (as_truncate ast))
 let all_credentials_ok_tree_truncate #bytes #bl #tkt #asp #l ts ast =
   all_credentials_ok_left_right ts ast
 
-val all_credentials_ok_tree_extend: #bytes:Type0 -> {|bytes_like bytes|} -> #tkt:treekem_types bytes -> #asp:as_parameters bytes -> #l:nat -> ts:treesync bytes tkt l 0 -> ast:as_tokens bytes asp l 0 -> Lemma
+val all_credentials_ok_tree_extend: #bytes:Type0 -> {|bytes_like bytes|} -> #tkt:treekem_types bytes -> #asp:as_parameters bytes -> #l:nat -> ts:treesync bytes tkt l 0 -> ast:as_tokens bytes asp.token_t l 0 -> Lemma
   (requires all_credentials_ok ts ast)
   (ensures all_credentials_ok (tree_extend ts) (as_extend ast))
 let all_credentials_ok_tree_extend #bytes #bl #tkt #asp #l ts ast =
@@ -114,7 +114,7 @@ let as_parameters_weaker #bytes #bl as_strong as_weak =
   as_strong.token_t == as_weak.token_t /\
   (forall vk cred token. as_strong.credential_ok (vk, cred) token ==> as_weak.credential_ok (vk, cred) token)
 
-val all_credentials_ok_weaken: #bytes:Type0 -> {|bytes_like bytes|} -> #tkt:treekem_types bytes -> #asp_strong:as_parameters bytes -> #l:nat -> #i:tree_index l -> asp_weak:as_parameters bytes -> ts:treesync bytes tkt l i -> ast:as_tokens bytes asp_strong l i -> Pure (as_tokens bytes asp_weak l i)
+val all_credentials_ok_weaken: #bytes:Type0 -> {|bytes_like bytes|} -> #tkt:treekem_types bytes -> #asp_strong:as_parameters bytes -> #l:nat -> #i:tree_index l -> asp_weak:as_parameters bytes -> ts:treesync bytes tkt l i -> ast:as_tokens bytes asp_strong.token_t l i -> Pure (as_tokens bytes asp_weak.token_t l i)
   (requires all_credentials_ok ts ast /\ as_parameters_weaker asp_strong asp_weak)
   (ensures fun res -> all_credentials_ok ts res)
 let all_credentials_ok_weaken #bytes #bl #tkt #asp_strong #l #i asp_weak ts ast =
